argumento implicito de trie0 a explicito y convención de nombres

Trie.fst
@@ -9,11 +9,11 @@ let alphabet_size : U32.t = U32.uint_to_t 26
 type b_nat = x:nat{x < U32.v alphabet_size /\ U.size x 32}
 
 noeq
-type trie0 (#n : U32.t) =
+type trie0 (n : U32.t) =
   | L
-  | N of raw (trie0 #n) n & bool & int
+  | N of raw (trie0 n) n & bool & int
 
-let rec mem (t : trie0 #alphabet_size) (l : list b_nat) : Tot bool (decreases l) =
+let rec mem (t : trie0 alphabet_size) (l : list b_nat) : Tot bool (decreases l) =
   match t with
   | L -> false
   | N (a, is_t, _) ->
@@ -24,20 +24,20 @@ let rec mem (t : trie0 #alphabet_size) (l : list b_nat) : Tot bool (decreases l)
       | L -> false
       | t' -> mem t' xs
 
-let empty_array : raw (trie0 #alphabet_size) alphabet_size =
+let empty_array : raw (trie0 alphabet_size) alphabet_size =
   init alphabet_size (fun _ -> L)
 
-let rec insert (t : trie0 #alphabet_size) (l: list b_nat) : Tot trie0 (decreases l) =
+let rec insert0 (t : trie0 alphabet_size) (l: list b_nat) : Tot (trie0 alphabet_size) (decreases l) =
   match (t,l) with
   | (L, []) -> N (empty_array, true, 0)
   | (N (a, _, n), []) -> N (a, true, n)
-  | (L, x::xs) -> N (init alphabet_size (fun i -> if i = x then insert L xs else L), false, 1)
+  | (L, x::xs) -> N (init alphabet_size (fun i -> if i = x then insert0 L xs else L), false, 1)
   | (N (a, b, n), x::xs) ->
     match index a (U32.uint_to_t x) with
-    | L -> N (update a (U32.uint_to_t x) (insert L xs), b, n + 1)
-    | t' -> N (update a (U32.uint_to_t x) (insert t' xs), b, n)
+    | L -> N (update a (U32.uint_to_t x) (insert0 L xs), b, n + 1)
+    | t' -> N (update a (U32.uint_to_t x) (insert0 t' xs), b, n)
 
-let rec delete (t : trie0 #alphabet_size) (l: list b_nat) : Tot (trie0 #alphabet_size) (decreases l) = 
+let rec delete0 (t : trie0 alphabet_size) (l: list b_nat) : Tot (trie0 alphabet_size) (decreases l) =
   match (t,l) with
   | (L, _) -> L
   | (N (_, _, 0), []) -> L
@@ -46,7 +46,7 @@ let rec delete (t : trie0 #alphabet_size) (l: list b_nat) : Tot (trie0 #alphabet
       match index a (U32.uint_to_t x) with
       | L -> N (a, is_t, n)
       | t' ->
-        match delete t' xs with
+        match delete0 t' xs with
         | L -> if n = 1 && not is_t
                then L
                else N (update a (U32.uint_to_t x) L , is_t, n-1)
